compiler/bootstrap/compilation/x64/64/proofs/x64BootstrapProofScript.sml
@@ -89,11 +89,10 @@ val compile_correct_applied =
   |> DISCH(#1(dest_imp(concl x64_init_ok)))
   |> REWRITE_RULE[AND_IMP_INTRO]
 
-val cake_compiled_thm =
+Theorem cake_compiled_thm =
   CONJ compile_correct_applied cake_output
   |> DISCH_ALL
- (* |> check_thm *)
-  |> curry save_thm "cake_compiled_thm";
+  |> check_thm;
 
 (* --- *)
 
